Prove that deleting an element decreases the size of 1
We proved that removing the minimal element from a priority queue decreases its size of 1. To do that, we simplified the definition of size and showed that the size of queue is the cardinal of the image of this queue by b_heap_to_bag.

translator/okasaki-examples/SkewBinomialHeapScript.sml
@@ -2,7 +2,6 @@
   Bootstrapped Skew Binomial Heaps, based on Purely Functional Data Structures
   sections 9.3.2 and 10.2.2 (Chris Okasaki)
 *)
-
 open preamble;
 open bagTheory bagLib;
 
@@ -121,6 +120,7 @@ val delete_min_def = Define `
               (merge_tree geq (REVERSE (children min)) (normalize geq ts'))))
 `;
 
+
 (* Bootstraping Skew Binomial Heaps *)
 Datatype `bsbHeap = Bsbempty | Bsbheap 'a (bsbHeap sbHeap)`;
 
@@ -206,6 +206,22 @@ val b_heap_to_bag_def = Define `
   (b_heap_to_bag4 geq [] = {||}) /\
   (b_heap_to_bag4 geq (t::ts) = BAG_UNION (b_heap_to_bag2 geq t)
                                           (b_heap_to_bag4 geq ts))
+`;
+
+val bsize_def = Define `
+  (bsize Bsbempty = 0:num) /\
+  (bsize (Bsbheap a0 a1) = 1 + (bsize1 a1)) /\
+  (bsize1 [] = 0) /\
+  (bsize1 (a0::a1) =
+     (bsize2 a0) + (bsize1 a1)) /\
+  (bsize2 (Sbnode a0 a1 a2 a3) =
+     (bsize a0) + (bsize3 a2) + (bsize4 a3)) /\
+  (bsize3 [] = 0) /\
+  (bsize3 (a0::a1) =
+    (bsize a0) + (bsize3 a1)) /\
+  (bsize4 [] = 0) /\
+  (bsize4 (a0::a1) =
+    (bsize2 a0) + (bsize4 a1))
 `;
 
 val is_tree_ordered_def = Define `
@@ -338,24 +354,25 @@ Proof
   rw[tree_to_bag_def,BAG_INSERT_UNION]
 QED;
 
-val bsbHeap_size_def = fetch "-" "bsbHeap_size_def";
+(* val bsize_def = fetch "-" "bsize_def"; *)
 
 Theorem equiv_size1_size4:
-  !f h. bsbHeap4_size f h = bsbHeap1_size f h
+  !h. bsize4 h = bsize1 h
 Proof
   Induct_on `h`
-  >- rw[bsbHeap_size_def]
-  >- rw[bsbHeap_size_def]
+  >- rw[bsize_def]
+  >- rw[bsize_def]
 QED;
 
 Theorem tree_size_general:
-  !f r n l0 l. bsbHeap2_size f (Sbnode r n l0 l) =
-               1 + n + (bsbHeap_size f r) +
-               (bsbHeap3_size f l0) + (bsbHeap1_size f l)
+  !r n l0 l. bsize2 (Sbnode r n l0 l) =
+             (bsize r) +
+             (bsize3 l0) +
+             (bsize1 l)
 Proof
   Induct_on `l`
-  >- rw[bsbHeap_size_def]
-  >- rw[bsbHeap_size_def, equiv_size1_size4]
+  >- rw[bsize_def]
+  >- rw[bsize_def, equiv_size1_size4]
 QED;
 
 Theorem reverse_bag:
@@ -447,43 +464,28 @@ Proof
 QED;
 
 Theorem elem_list_size:
-  !f x l. BAG_IN x (LIST_TO_BAG l) ==>
-          bsbHeap_size f x < 1 + (bsbHeap3_size f l)
+  !x l. BAG_IN x (LIST_TO_BAG l) ==>
+          bsize x < 1 + (bsize3 l)
 Proof
   Induct_on `l`
   >- rw[LIST_TO_BAG_def]
-  >- (rw[LIST_TO_BAG_def, bsbHeap_size_def]
+  >- (rw[LIST_TO_BAG_def, bsize_def]
       >- decide_tac
       >- (res_tac \\
-          pop_assum (qspecl_then [`f`] mp_tac) \\
           decide_tac))
 QED;
 
-Theorem head_heap_size:
-  !f t h. bsbHeap2_size f t < bsbHeap1_size f (t::h)
-Proof
-  rw[bsbHeap_size_def]
-QED;
-
-Theorem tree_first_child_size:
-  !f a n l c cs. bsbHeap2_size f c < bsbHeap2_size f (Sbnode a n l (c::cs))
-Proof
-  rw[bsbHeap_size_def]
-QED;
-
 Theorem elem_tree_size:
-  !f .(!t x. BAG_IN x (tree_to_bag t) ==>
-        bsbHeap_size f x < 1 + (bsbHeap2_size f t)) /\
-      (!ts x. BAG_IN x (heap_to_bag ts) ==>
-        bsbHeap_size f x < 1 + (bsbHeap4_size f ts))
+  (!(t: 'a bsbHeap sbTree) x. BAG_IN x (tree_to_bag t) ==>
+    bsize x < 1 + (bsize2 t)) /\
+  (!(ts: 'a bsbHeap sbHeap) x. BAG_IN x (heap_to_bag ts) ==>
+    bsize x < 1 + (bsize4 ts))
 Proof
-  strip_tac \\
   ho_match_mp_tac (fetch "-" "sbTree_induction") \\
   rw[]
   >- (fs[tree_to_bag_def] \\
       EVAL_TAC \\ fs[]
       >- (imp_res_tac elem_list_size \\
-          pop_assum (qspecl_then [`f`] mp_tac) \\
           rw[])
       >- (res_tac \\
           rw[]))
@@ -2082,13 +2084,100 @@ Proof
               metis_tac[COMM_BAG_UNION, ASSOC_BAG_UNION])))
 QED;
 
+val bsbHeap_ind  = fetch "-" "bsbHeap_induction";
+
+Theorem b_finite_bag:
+  !geq.
+    TotalPreOrder geq ==>
+    (!(h: 'a bsbHeap). FINITE_BAG (b_heap_to_bag geq h)) /\
+    (!(l: 'a bsbHeap sbTree list). FINITE_BAG (b_heap_to_bag1 geq l)) /\
+    (!(s: 'a bsbHeap sbTree). FINITE_BAG (b_heap_to_bag2 geq s)) /\
+    (!(l: 'a bsbHeap list). FINITE_BAG (b_heap_to_bag3 geq l)) /\
+    (!(l: 'a bsbHeap sbTree list). FINITE_BAG (b_heap_to_bag4 geq l))
+Proof
+  ntac 2 strip_tac \\
+  ho_match_mp_tac bsbHeap_ind \\ rw[] \\
+  rw[b_heap_to_bag_def]
+QED;
+
+Theorem b_size_bag_card:
+  !geq. TotalPreOrder geq ==>
+        (!h. is_b_heap_ordered geq h ==>
+             bsize h =
+             BAG_CARD (b_heap_to_bag geq h)) /\
+        (!l. is_b_heap_ordered1 geq l ==>
+             bsize1 l =
+             BAG_CARD (b_heap_to_bag1 geq l)) /\
+        (!s. is_b_heap_ordered2 geq s ==>
+             bsize2 s =
+             BAG_CARD (b_heap_to_bag2 geq s)) /\
+        (!l. is_b_heap_ordered3 geq l ==>
+             bsize3 l =
+	     BAG_CARD (b_heap_to_bag3 geq l)) /\
+        (!l. is_b_heap_ordered4 geq l ==>
+             bsize4 l =
+             BAG_CARD (b_heap_to_bag4 geq l))
+Proof
+  ntac 2 strip_tac \\
+  ho_match_mp_tac bsbHeap_ind \\
+  rw[b_heap_to_bag_def, bsize_def] \\
+  fs[is_b_heap_ordered_def]
+  >- metis_tac[b_finite_bag, BAG_CARD_THM]
+  >- (`FINITE_BAG (b_heap_to_bag2 geq s)` by metis_tac[b_finite_bag] \\
+      `FINITE_BAG (b_heap_to_bag1 geq l)` by metis_tac[b_finite_bag] \\
+      imp_res_tac BAG_CARD_UNION \\
+      rw[])
+  >- (`FINITE_BAG (b_heap_to_bag geq h)` by metis_tac[b_finite_bag] \\
+      `FINITE_BAG (b_heap_to_bag3 geq l)` by metis_tac[b_finite_bag] \\
+      `FINITE_BAG (b_heap_to_bag4 geq l')` by metis_tac[b_finite_bag] \\
+      imp_res_tac BAG_CARD_UNION \\
+      rw[])
+  >- (`FINITE_BAG (b_heap_to_bag geq h)` by metis_tac[b_finite_bag] \\
+      `FINITE_BAG (b_heap_to_bag3 geq l)` by metis_tac[b_finite_bag] \\
+      imp_res_tac BAG_CARD_UNION \\
+      rw[])
+  >- (`FINITE_BAG (b_heap_to_bag2 geq s)` by metis_tac[b_finite_bag] \\
+      `FINITE_BAG (b_heap_to_bag4 geq l)` by metis_tac[b_finite_bag] \\
+      imp_res_tac BAG_CARD_UNION \\
+      rw[])
+QED;
+
+Theorem b_delete_size:
+  !geq h. TotalPreOrder geq /\
+          h <> Bsbempty /\
+          is_b_heap_ordered geq h ==>
+	  bsize h =
+          bsize (THE (b_delete_min geq h)) + 1
+Proof
+  rpt strip_tac \\
+  imp_res_tac b_delete_min_order \\
+  WEAKEN_TAC is_imp \\
+  `bsize h = BAG_CARD (b_heap_to_bag geq h)` by
+  metis_tac[b_size_bag_card] \\
+  `bsize (THE (b_delete_min geq h)) =
+   BAG_CARD (b_heap_to_bag geq (THE (b_delete_min geq h)))` by
+  metis_tac[b_size_bag_card] \\
+  fs[] \\
+  Cases_on `h`
+  >- fs[]
+  >- (imp_res_tac b_delete_min_correct \\ fs[] \\
+      rw[b_find_min_def] \\
+      `FINITE_BAG (b_heap_to_bag geq (THE (b_delete_min geq (Bsbheap a l))))` by
+      metis_tac[b_finite_bag] \\
+      `FINITE_BAG {|a|}` by fs[] \\
+      rw [BAG_CARD_UNION] \\
+      `BAG_CARD {| a |} = 1` suffices_by fs[] \\
+      `FINITE_BAG {||}` by fs[] \\
+      rw[BAG_CARD_THM])
+QED;
+
 open ListProgTheory ml_translatorTheory;
 open ml_translatorLib;
 
 val _ = translation_extends "ListProg";
 
-val _ = register_type ``:'a sbTree``;
-(* val _ = register_type ``:'a sbHeap``; *)
+
+ val _ = register_type ``:'a sbTree``;
 
 val _ = translate leaf_def;
 val _ = translate root_def;
@@ -2128,14 +2217,15 @@ val SKEWBINOMIALHEAP_BSBHEAP_TYPE_def = tDefine "SKEWBINOMIALHEAP_BSBHEAP_TYPE" 
                        ARB) x_1 v2_2) ∧
   (SKEWBINOMIALHEAP_BSBHEAP_TYPE a Bsbempty v ⇔
     v = Conv (SOME (TypeStamp "Bsbempty" 6)) [])`
-  (WF_REL_TAC `measure ((bsbHeap_size (K 0)) o FST o SND)`
+  (WF_REL_TAC `measure (bsize o FST o SND)`
    \\ REPEAT STRIP_TAC
    \\ TRY (PAT_X_ASSUM (MEM |> CONJUNCT2 |> SPEC_ALL |> concl |> rand |> rand)
       (fn th => ASSUME_TAC th THEN Induct_on [ANTIQUOTE (rand (rand (concl th)))]))
    \\ FULL_SIMP_TAC std_ss [MEM,FORALL_PROD,size_def] \\ REPEAT STRIP_TAC \\
    imp_res_tac elem_tree_size \\
-   pop_assum (qspecl_then [`(K 0)`] mp_tac) \\
-   fs[]>>
+   res_tac \\
+   (*  pop_assum (qspecl_then [`(K 0)`] mp_tac) \\ *)
+   fs[bsize_def]>>
    EVAL_TAC \\ rw[]);
 
 val SKEWBINOMIALHEAP_SBTREE_TYPE_def = theorem "SKEWBINOMIALHEAP_SBTREE_TYPE_def";
